\documentclass[a4paper,10pt]{article}
%\documentclass[a4paper,10pt]{scrartcl}

\usepackage[utf8]{inputenc}
\usepackage{datetime2}
\usepackage{amsmath}

\title{Derivation of Spiral Endpoint}
\author{Willow Herron}


\begin{document}
	\maketitle
	\tiny \begin{align*}
		r_0(\theta) &= a(\theta-d)^3-b(\theta-d)\\
		r_1(\theta) &= a(\theta-e)^3-c(\theta-e)\\
		r_0 &= r_1\\
		(\theta-d)(a(\theta-d)^2-b) &= (\theta-e)(a(\theta-e)^2-c)\\
		(\theta-d)(a\theta^2-2ad\theta+(ad^2-b)) &= (\theta-e)(a\theta^2-2ae\theta+(ae^2-c))\\
		-3ad\theta^2+(3ad^2-b)\theta-d(ad^2-b)&=-3ae\theta^2+(3ae^2-c)\theta-e(ae^2-c)\\
		0 &= 3a(e-d)\theta^2+(3a(d^2-e^2)-b+c)\theta-ad^3+bd+ae^3-ce\\
		x &= \frac{3a(e^2-d^2)+b-c\pm\sqrt{(3a(d^2-e^2)-b+c)^2-12a(e-d)(ae^3-ce-ad^3+bd)}}{6a(e-d)}
	\end{align*}
\end{document}
